progessing

ML_SP_Eval.v
@@ -7,7 +7,11 @@ Set Implicit Arguments.
 
 Require Import Arith List Metatheory.
 Require Import ML_SP_Definitions ML_SP_Infrastructure.
-Require Import ML_SP_Soundness.
+Require Import ML_SP_Soundness ML_SP_Unify ML_SP_Rename.
+
+Ltac case_rewrite H t :=
+  case_eq t; introv H; rewrite H in *; try discriminate.
+
 
 Section ListForall.
 Variables (A:Set) (P:A->Prop).
@@ -44,8 +48,9 @@ Hint Resolve list_forall_apply.
 
 Module MkEval(Cstr:CstrIntf)(Const:CstIntf).
 
-Module Sound := MkSound(Cstr)(Const).
-Import Sound.
+Module Rename := MkRename(Cstr)(Const).
+Import Rename.
+Import Unify.Sound.
 Import Infra.
 Import Defs.
 Import Metatheory_Env.Env.
@@ -189,6 +194,21 @@ Fixpoint cut (n:nat) (l:list A) {struct n} : list A * list A :=
     | a :: l => let (l1, l2) := cut n l in (a :: l1, l2)
     end
   end.
+
+Lemma cut_ok : forall n l l1 l2,
+  n <= length l -> cut n l = (l1, l2) ->
+  length l1 = n /\ l = l1 ++ l2.
+Proof.
+  induction n; simpl; intros.
+    inversions* H0.
+  destruct l; simpl in *.
+    elimtype False; omega.
+  assert (n <= length l) by omega.
+  case_rewrite R (cut n l).
+  inversions* H0.
+  destruct* (IHn l l0 l2).
+  subst*.
+Qed.
 End Cut.
 
 Parameter delta_red : Const.const -> list clos -> clos.
@@ -281,15 +301,16 @@ Fixpoint eval (h:nat) (benv:list clos) (app:list clos) (t:trm)
       let nargs := length l +  length app in
         let nred := S(Const.arity cst) in
         if le_lt_dec nred nargs then
-        let (args, app') := cut nred (List.app l app) in
-        match delta_red cst args with
-        | clos_const cst' app'' =>
-          eval h nil (List.app app'' app') (trm_cst cst') stack
-        | clos_abs t1 benv =>
-          eval h benv app' (trm_abs t1) stack
-        end
-      else result c
-    end end end
+          let (args, app') := cut nred (List.app l app) in
+          match delta_red cst args with
+          | clos_const cst' app'' =>
+            eval h nil (List.app app'' app') (trm_cst cst') stack
+          | clos_abs t1 benv =>
+            eval h benv app' (trm_abs t1) stack
+          end
+        else result (clos_const cst (l++app))
+      end
+    end end
   end.
 End Eval.
 
@@ -319,22 +340,27 @@ Definition skk' := eval nil 3 nil nil
 Eval compute in skk'.
 Eval compute in res2trm skk'.
 
-Module Sound2 := Sound.Mk2(Delta).
-Import Sound2.
+Module Rename2 := Rename.Mk2(Delta).
+Import Rename2.
+Import Sound.
 Import JudgInfra.
 Import Judge.
 
-Parameter delta_red_sound : forall c cls K T,
-  length cls = (S(Const.arity c)) ->
-  K ; empty |(false,GcLet)|= const_app c (List.map clos2trm cls) ~: T ->
+Definition gc := (false, GcAny).
+
+Parameter delta_red_sound : forall c cls,
+  list_for_n clos_ok (S(Const.arity c)) cls ->
   exists t1:trm, exists t2:trm, exists tl:list trm,
-    Delta.rule (length tl) t1 t2 /\ list_forall term tl /\
-    const_app c (List.map clos2trm cls) = trm_inst t1 tl /\
-    clos2trm (delta_red c cls) = trm_inst t2 tl.
+    forall K E T,
+      K ; E |gc|= const_app c (List.map clos2trm cls) ~: T ->
+      Delta.rule (length tl) t1 t2 /\ list_forall term tl /\
+      const_app c (List.map clos2trm cls) = trm_inst t1 tl /\
+      clos2trm (delta_red c cls) = trm_inst t2 tl /\
+      clos_ok (delta_red c cls).
 
 Module Mk3(SH:SndHypIntf).
 
-Module Sound3 := Sound2.Mk3(SH).
+Module Sound3 := Sound.Mk3(SH).
 Import Sound3.
 
 Lemma clos_ok_value : forall cl,
@@ -374,23 +400,6 @@ Proof.
     rewrite* IHt.
    rewrite IHt1; rewrite* IHt2.
   rewrite IHt1; rewrite* IHt2.
-Qed.
-
-Definition gc := (false, GcAny).
-
-Lemma typing_app_abs_let : forall K E t1 t2 T,
-  K; E |gc|= trm_app (trm_abs t2) t1 ~: T ->
-  K; E |gc|= trm_let t1 t2 ~: T.
-Proof.
-  intros.
-  inversions H; try discriminate; simpl in *.
-  inversions H4; try discriminate; simpl in *.
-  apply (@typing_let gc (Sch S nil) {} L).
-    simpl; intros.
-    destruct Xs; try elim H0.
-    unfold kinds_open_vars, kinds_open, sch_open_vars; simpl.
-    rewrite* typ_open_vars_nil.
-  apply H8.
 Qed.
 
 Lemma term_trm_inst : forall n t tl,
@@ -434,8 +443,37 @@ Qed.
 Definition is_abs t :=
   match t with trm_abs _ => true | _ => false end.
 
+Lemma app_trm_cases : forall t1,
+  (forall t2, app_trm t1 t2 = trm_app t1 t2) \/ (exists t, t1 = trm_abs t).
+Proof.
+  intros.
+  destruct t1; simpl*.
+Qed.
+
+Lemma app_trm_false : forall t1 t2,
+  is_abs t1 = false -> app_trm t1 t2 = trm_app t1 t2.
+Proof.
+  intros.
+  destruct* (app_trm_cases t1).
+  destruct H0; subst; discriminate.
+Qed.
+
 Definition retypable t1 t2 :=
   forall K E T, K; E |gc|= t1 ~: T -> K; E |gc|= t2 ~: T.
+
+Lemma typing_app_abs_let : forall t1 t2,
+  retypable (trm_app (trm_abs t2) t1) (trm_let t1 t2).
+Proof.
+  intros; intro; intros.
+  inversions H; try discriminate; simpl in *.
+  inversions H4; try discriminate; simpl in *.
+  apply (@typing_let gc (Sch S nil) {} L).
+    simpl; intros.
+    destruct Xs; try elim H0.
+    unfold kinds_open_vars, kinds_open, sch_open_vars; simpl.
+    rewrite* typ_open_vars_nil.
+  apply H8.
+Qed.
 
 Lemma trm_open_comm : forall i j u v t,
   i <> j -> term u -> term v ->
@@ -501,16 +539,6 @@ Proof.
   intros; intro; intros.
   unfold app_trm; destruct* t1.
   apply* typing_app_abs_let.
-Qed.
-
-Ltac case_rewrite H t :=
-  case_eq t; introv H; rewrite H in *; try discriminate.
-
-Lemma app_trm_cases : forall t1,
-  (forall t2, app_trm t1 t2 = trm_app t1 t2) \/ (exists t, t1 = trm_abs t).
-Proof.
-  intros.
-  destruct t1; simpl*.
 Qed.
 
 Hint Resolve term_closed_0 clos_ok_term.
@@ -584,18 +612,15 @@ Proof.
 Qed.
 
 Lemma retypable_app_trm : forall t1 t2 t3 t4,
-  term t1 -> term t2 -> is_abs t1 = false ->
+  is_abs t1 = false ->
   retypable t1 t2 -> retypable t3 t4 ->
   retypable (app_trm t1 t3) (app_trm t2 t4).
 Proof.
   intros.
-  destruct (app_trm_cases t1).
-    rewrite H4.
-    clear H4; intro; intros.
-    apply* retypable_trm_app.
-    inversions* H4; discriminate.
-  destruct H4.
-  subst; discriminate.
+  rewrite (app_trm_false _ _ H).
+  intro; intros.
+  apply* retypable_trm_app.
+  inversions* H2; discriminate.
 Qed.
 
 Lemma is_abs_app_trm : forall t1 t2,
@@ -612,17 +637,23 @@ Proof.
   rewrite map_app. rewrite* fold_left_app.
 Qed.
 
+Lemma is_abs_fold_left_app_trm : forall t args,
+  is_abs t = false -> is_abs (fold_left app_trm args t) = false.
+Proof.
+  intros; induction args using rev_ind. auto.
+  rewrite fold_left_app. simpl. apply is_abs_app_trm.
+Qed.
+
 Lemma is_abs_app2trm : forall t args,
   is_abs t = false -> is_abs (app2trm t args) = false.
 Proof.
-  intros; induction args using rev_ind. auto.
-  rewrite app2trm_app. unfold app2trm at 1. simpl. apply is_abs_app_trm.
+  intros; unfold app2trm. apply* is_abs_fold_left_app_trm.
 Qed.
 
 Hint Resolve term_app_trm term_app2trm.
 
 Lemma retypable_app2trm : forall t1 t2 args,
-  term t1 -> term t2 -> is_abs t1 = false ->
+  is_abs t1 = false ->
   retypable t1 t2 ->
   list_forall clos_ok args ->
   retypable (app2trm t1 args) (app2trm t2 args).
@@ -630,7 +661,7 @@ Proof.
   intros; induction args using rev_ind. auto.
   repeat rewrite app2trm_app.
   assert (list_forall clos_ok args).
-    apply list_forall_in; intros; apply* (list_forall_out H3).
+    apply list_forall_in; intros; apply* (list_forall_out H1).
   unfold app2trm at 1 3. simpl.
   apply retypable_app_trm; auto.
    apply* is_abs_app2trm.
@@ -638,18 +669,16 @@ Proof.
 Qed.
 
 Lemma retypable_stack2trm : forall t1 t2 fl,
-  term t1 -> term t2 -> is_abs t1 = false ->
+  term t1 -> is_abs t1 = false ->
   retypable t1 t2 ->
   list_forall frame_ok fl ->
   retypable (stack2trm t1 fl) (stack2trm t2 fl).
 Proof.
   intros.
-  gen t1 t2; induction H3; intros; simpl. auto.
+  gen t1 t2; induction H2; intros; simpl. auto.
   destruct x as [benv app t'].
   case_eq (is_bvar t1); intros.
     inversions H0; discriminate.
-  case_eq (is_bvar t2); intros.
-    inversions H2; discriminate.
   inversions H; clear H.
   assert (Ht': term (trm_inst t' (List.map clos2trm benv))).
     apply term_trm_inst_closed.
@@ -663,20 +692,155 @@ Proof.
   destruct (app_trm_cases (trm_inst t' (List.map clos2trm benv))).
     do 2 rewrite H; clear H.
     intro; intros.
-    inversions* H; try discriminate.
+    inversions H; try discriminate.
+    case_eq (is_bvar t2); intros.
+      poses Ht2 (proj43 (typing_regular (H3 _ _ _ H14))).
+      inversions Ht2; discriminate.
+    auto*.
   destruct H. subst; rewrite H in *; simpl.
   intro; intros.
-  inversions* H7; try discriminate.
+  inversions H5; try discriminate.
+  case_eq (is_bvar t2); intros.
+    destruct (var_freshes L1 (sch_arity M)).
+    poses Ht2 (proj43 (typing_regular (H3 _ _ _ (H13 _ f)))).
+    inversions Ht2; discriminate.
+  auto*.
 Qed.
 
-Theorem eval_sound : forall h fl benv args K E t T,
+Lemma term_fold_app : forall tl t,
+  list_forall term tl -> term t -> term (fold_left trm_app tl t).
+Proof.
+  intros; gen t.
+  induction H; intros; simpl*.
+Qed.
+
+Lemma typing_app_trm_inv : forall K E t1 t2 T,
+  is_abs t1 = false ->
+  K; E |gc|= app_trm t1 t2 ~: T ->
+  exists T1, K; E |gc|= t1 ~: T1.
+Proof.
+  intros.
+  rewrite (app_trm_false _ _ H) in H0.
+  inversions* H0; try discriminate.
+Qed.
+
+Lemma typing_app2trm_inv : forall K E t1 cl T,
+  K; E |gc|= app2trm t1 cl ~: T ->
+  is_abs t1 = false ->
+  exists T1, K; E |gc|= t1 ~: T1.
+Proof.
+  unfold app2trm.
+  intros.
+  gen T; induction (List.map clos2trm cl) using rev_ind; simpl; intros.
+    auto*.
+  rewrite fold_left_app in H.
+  simpl in H.
+  destruct* (typing_app_trm_inv _ _ (is_abs_fold_left_app_trm _ l H0)  H).
+Qed.
+
+Lemma is_bvar_app_trm : forall t1 t2, is_bvar (app_trm t1 t2) = false.
+Proof. 
+  intros; destruct (app_trm_cases t1).
+    rewrite* H.
+  destruct H; rewrite* H.
+Qed.
+Hint Resolve is_bvar_app_trm.
+
+Lemma typing_stack2trm_inv : forall K E fl t1 T,
+  K; E |gc|= stack2trm t1 fl ~: T ->
+  is_bvar t1 = false ->
+  exists T1, exists K, K; E |gc|= t1 ~: T1.
+Proof.
+  induction fl; simpl; intros. auto*.
+  destruct a as [benv args t].
+  rewrite H0 in H.
+  destruct (IHfl _ _ H) as [T1 [K' Typ]].
+    clear.
+    unfold app2trm. induction (List.map clos2trm args) using rev_ind.
+      simpl*.
+    rewrite fold_left_app; simpl*.
+  clear -H0 Typ.
+  set (t0 := trm_inst t (List.map clos2trm benv)) in *.
+  destruct (typing_app2trm_inv _ _ Typ).
+    apply is_abs_app_trm.
+  destruct (app_trm_cases t0).
+    rewrite H1 in H; inversions* H; try discriminate.
+  destruct H1; rewrite H1 in H.
+  inversions* H; try discriminate.
+  destruct (var_freshes L1 (sch_arity M)).
+  auto*.
+Qed.
+
+Lemma app2trm_cases : forall t cl,
+  (exists t1, exists t2, app2trm t cl = trm_app t1 t2) \/
+  (exists t1, exists t2, app2trm t cl = trm_let t1 t2) \/
+  app2trm t cl = t.
+Proof.
+  intros.
+  induction cl using rev_ind. simpl*.
+  rewrite app2trm_app.
+  destruct (app_trm_cases (app2trm t cl)); unfold app2trm at 1 3; simpl.
+    rewrite* H.
+  destruct H; rewrite H. simpl*.
+Qed.
+
+Lemma app2trm_cst : forall c cl,
+  app2trm (trm_cst c) cl = const_app c (List.map clos2trm cl).
+Proof.
+  unfold app2trm, const_app.
+  induction cl using rev_ind. simpl*.
+  rewrite map_app. repeat rewrite fold_left_app. simpl.
+  rewrite app_trm_false. rewrite* IHcl.
+  apply* is_abs_app2trm.
+Qed.
+
+Section Eval.
+
+Variables (E:Defs.env) (fenv:env clos).
+
+Hypothesis E_ok : env_ok E.
+
+Hypothesis fenv_ok : forall x M,
+  binds x M E ->
+  exists cl, binds x cl fenv /\
+    has_scheme_vars gc {} empty empty (clos2trm cl) M.
+
+Lemma concat_empty : forall (A:Set) (K:env A), empty & K = K.
+Proof. intros; symmetry; apply (app_nil_end K). Qed.
+
+Lemma has_scheme_from_vars' : forall K t M,
+  has_scheme_vars gc {} empty empty t M ->
+  kenv_ok K -> env_ok E ->
+  has_scheme gc K E t M.
+Proof.
+  clear fenv_ok.
+  intros.
+  apply (@has_scheme_from_vars gc (dom K)).
+  intro; intros.
+  replace K with (empty & K) by apply concat_empty.
+  apply typing_weaken_kinds.
+    replace E with (empty & E & empty) by (simpl; apply concat_empty).
+    apply typing_weaken.
+      simpl.
+      apply* H.
+    simpl. rewrite* concat_empty.
+  assert (fresh {} (sch_arity M) Xs) by auto.
+  puts (H _ H3).
+  rewrite concat_empty.
+  rewrite concat_empty in H4.
+  apply* kenv_ok_concat.
+  rewrite* dom_kinds_open_vars.
+  apply* fresh_disjoint.
+Qed.
+
+Theorem eval_sound : forall h fl benv args K t T,
   list_forall clos_ok args ->
   list_forall clos_ok benv ->
   closed_n (length benv) t ->
   list_forall frame_ok fl ->
   K ; E |gc|=
     stack2trm (app2trm (trm_inst t (List.map clos2trm benv)) args) fl ~: T ->
-  K ; E |gc|= res2trm (eval nil h benv args t fl) ~: T.
+  K ; E |gc|= res2trm (eval fenv h benv args t fl) ~: T.
 Proof.
   induction h; introv; intros Hargs Hbenv Ht Hfl Typ.
     simpl*.
@@ -688,7 +852,7 @@ Proof.
         destruct fl.
          clear IHh. simpl in *.
          destruct (le_lt_dec (length (List.map clos2trm benv)) n).
-           rewrite nth_overflow in Typ; auto. inversions Typ. inversion H.
+          rewrite nth_overflow in Typ; auto. inversions Typ. inversion H.
          rewrite <- (nth_indep _ (clos2trm clos_def) (trm_bvar n) l) in Typ.
          rewrite map_nth in Typ. auto.
         destruct f as [benv' app' t'].
@@ -700,20 +864,20 @@ Proof.
         rewrite (nth_indep _ (trm_bvar n) (clos2trm clos_def) H2) in Typ.
         rewrite map_nth in Typ.
         assert (Hn: clos_ok (nth n benv clos_def)).
-          apply (list_forall_out Hbenv).
-          apply* nth_In.
+         apply (list_forall_out Hbenv).
+         apply* nth_In.
         simpl in Typ.
         case_rewrite R (is_bvar (clos2trm (nth n benv clos_def))).
-          case_rewrite R1 (clos2trm (nth n benv clos_def)).
-          clear -R1 Hn.
-          assert (term (trm_bvar n0)).
-            rewrite <- R1.
-            apply* clos_ok_term.
-          inversion H.
+         case_rewrite R1 (clos2trm (nth n benv clos_def)).
+         clear -R1 Hn.
+         assert (term (trm_bvar n0)).
+          rewrite <- R1.
+          apply* clos_ok_term.
+         inversion H.
         clear R.
         set (t1 := trm_inst t' (List.map clos2trm benv')) in *.
         replace (app2trm (app_trm t1 (clos2trm (nth n benv clos_def))) app')
-           with (app2trm t1 (nth n benv clos_def :: app')) in Typ; auto*.
+          with (app2trm t1 (nth n benv clos_def :: app')) in Typ; auto*.
        simpl trm2clos.
        case_eq (nth n benv clos_def); intros.
         inversions Hargs; clear Hargs.
@@ -732,33 +896,17 @@ Proof.
         rewrite map_nth in Typ.
         rewrite H in Typ.
         simpl in Typ.
-        refine (retypable_stack2trm _ _ _ _ _ Typ); auto.
-           apply* term_app2trm.
-           rewrite <- (@term_trm_inst 0 (clos2trm arg) (List.map clos2trm l)).
-            change (term (trm_inst (trm_let (clos2trm arg) t)
-                             (List.map clos2trm l))).
-            apply term_trm_inst_closed.
-             rewrite* map_length.
-            apply* list_forall_map.
-           auto.
+        refine (retypable_stack2trm _ _ _ _ Typ); auto.
           apply* term_app2trm.
-          apply term_trm_inst_closed.
-           simpl; rewrite* map_length.
-          constructor; auto.
-          apply* list_forall_map.
-         apply* is_abs_app2trm.
-        apply* retypable_app2trm. 
           rewrite <- (@term_trm_inst 0 (clos2trm arg) (List.map clos2trm l)).
            change (term (trm_inst (trm_let (clos2trm arg) t)
-                             (List.map clos2trm l))).
+                            (List.map clos2trm l))).
            apply term_trm_inst_closed.
             rewrite* map_length.
            apply* list_forall_map.
           auto.
-         apply term_trm_inst_closed.
-         simpl; rewrite* map_length.
-         constructor; auto.
-         apply* list_forall_map.
+         apply* is_abs_app2trm.
+        apply* retypable_app2trm.
         intro; intros.
         clear Typ; inversions H0; try discriminate.
         unfold trm_inst, trm_open in H12.
@@ -784,46 +932,153 @@ Proof.
         simpl.
         case_eq (l ++ arg :: args); intros. destruct l; discriminate.
         case_eq (cut (Const.arity c) l1); intros.
-        case_eq (delta_red c (c0 :: l2)); intros.
-      
+        unfold trm_inst in Typ; simpl in Typ.
+        rewrite <- minus_n_O in Typ.
+        rewrite <- (nth_indep _ (clos2trm clos_def)) in Typ;
+          [|rewrite map_length; inversions* Ht].
+        rewrite map_nth in Typ.
+        rewrite H in Typ; simpl in Typ.
+        assert (Const.arity c <= length l1).
+         clear -l0 H0.
+         puts (f_equal (@length clos) H0).
+         rewrite app_length in H.
+         simpl in H.
+         omega.
+        destruct (cut_ok _ H2 H1).
+        replace (app2trm (const_app c (List.map clos2trm l)) (arg :: args))
+          with (app2trm (const_app c (List.map clos2trm (c0 :: l2))) l3)
+            in Typ.
+         subst.
+         assert (Hok: list_forall clos_ok (c0 :: l2 ++ l3)).
+          rewrite <- H0.
+          apply list_forall_in.
+          intros.
+          destruct (in_app_or _ _ _ H4).
+           assert (clos_ok (clos_const c l)).
+            rewrite <- H.
+            apply (list_forall_out Hbenv).
+            inversions Ht.
+            apply* nth_In.
+           inversions H6; clear H6.
+           apply* (list_forall_out H9).
+          apply* (list_forall_out Hargs).
+         assert (Hok2: list_forall clos_ok (c0 :: l2)).
+          apply list_forall_in; intros; apply* (list_forall_out Hok).
+         assert (Hok3: list_forall clos_ok l3).
+          apply list_forall_in; intros; apply* (list_forall_out Hok).
+         destruct (@delta_red_sound c (c0 :: l2))
+           as [t1 [t2 [tl Hd]]].
+           split*. simpl; rewrite* H3.
+         assert (K; E |gc|=
+           stack2trm (app2trm (clos2trm (delta_red c (c0 :: l2))) l3) fl ~: T).
+          assert (Habs: forall l, is_abs (const_app c l) = false).
+           clear; unfold const_app.
+           induction l using rev_ind.
+            simpl*.
+           rewrite fold_left_app. simpl*.
+          refine (retypable_stack2trm _ _ _ _ Typ); auto.
+            apply* term_app2trm.
+            unfold const_app. apply* term_fold_app.
+            apply* (@list_forall_map _ _ clos2trm clos_ok).
+           apply* is_abs_app2trm.
+          apply* retypable_app2trm.
+          intro; intros.
+          destruct (Hd _ _ _ H4) as [Hr [Htl [Ht1 [Ht2 _]]]]; clear Typ Hd.
+          rewrite Ht1 in H4.
+          rewrite Ht2.
+          apply* SH.delta_typed. split*.
+         assert (clos_ok (delta_red c (c0 :: l2))).
+          clear -Typ Hd.
+          set (args := List.map clos2trm (c0 :: l2)) in *.
+          destruct (typing_stack2trm_inv _ _ Typ).
+           destruct (app2trm_cases (const_app c args) l3).
+            destruct H as [t1' [t2' Happ]]. rewrite* Happ.
+           destruct H.
+            destruct H as [t1' [t2' Happ]]. rewrite* Happ.
+           rewrite H. unfold const_app.
+           clear. induction args using rev_ind.
+            simpl*.
+           rewrite fold_left_app. simpl*.
+          destruct H.
+          destruct (typing_app2trm_inv _ _ H).
+           clear. unfold const_app; induction args using rev_ind.
+            simpl*.
+           rewrite fold_left_app. simpl*.
+          destruct* (Hd _ _ _ H0).
+         case_rewrite R (delta_red c (c0 :: l2)).
+          inversions H5.
+          apply* IHh.
+         inversions H5.
+         apply* IHh.
+          apply* list_forall_app.
+         simpl in *.
+         rewrite trm_inst_nil.
+         rewrite app2trm_app.
+         rewrite* app2trm_cst.
+        do 2 rewrite <- app2trm_cst.
+        do 2 rewrite <- app2trm_app.
+        rewrite H0. simpl. rewrite* H4.
+       simpl.
+       assert (Hlen: n < length benv).
+        destruct* (le_lt_dec (length benv) n).
+        rewrite nth_overflow in H; auto. discriminate.
+       assert (Hn: trm_inst (trm_bvar n) (List.map clos2trm benv)
+                   = clos2trm (clos_const c l)).
+        unfold trm_inst; simpl.
+        rewrite <- minus_n_O.
+        rewrite <- (map_length clos2trm) in Hlen.
+        rewrite <- (nth_indep _ (clos2trm clos_def) (trm_bvar n) Hlen).
+        rewrite map_nth.
+        rewrite* H.
+       destruct fl.
+        simpl in *.
+        rewrite <- app2trm_cst.
+        rewrite app2trm_app.
+        rewrite app2trm_cst.
+        rewrite Hn in Typ. auto.
+       destruct f as [benv' app' t].
+       inversions Hfl; clear Hfl.
+       inversions H3; clear H3.
+       apply* IHh; clear IHh.
+        constructor; auto.
+        constructor.
+         apply* list_forall_app.
+         assert (clos_ok (clos_const c l)).
+          rewrite <- H.
+          apply (list_forall_out Hbenv).
+          apply* nth_In.
+         inversions* H0.
+        rewrite app_length; simpl; omega.
+       simpl in Typ.
+       rewrite Hn in Typ.
+       case_rewrite R (is_bvar
+                      (app2trm (clos2trm (clos_const c l)) (arg :: args))).
+        unfold app2trm in R.
+        clear -R; induction args using rev_ind; simpl in R.
+         rewrite is_bvar_app_trm in R. discriminate.
+        rewrite map_app in R; rewrite fold_left_app in R; simpl in R.
+        rewrite is_bvar_app_trm in R. discriminate.
+       simpl in Typ.
+       rewrite <- app2trm_cst in Typ.
+       rewrite <- app2trm_app in Typ.
+       unfold app2trm in Typ.
+       unfold app2trm; simpl.
+       rewrite <- app2trm_cst.
+       apply Typ.
+      destruct args as [|arg args].
+       destruct fl.
+        unfold app2trm, trm_inst in Typ.
+        clear -fenv_ok Typ.
+        simpl in *.
+        inversions Typ; try discriminate.
+        destruct (fenv_ok H2) as [cl [B Typ']].
+        rewrite B.
+        destruct H5.
+        apply* has_scheme_from_vars'.
+       
+
 End.
 
-Section Eval.
-
-Variables (K':kenv) (T':typ) (E':Defs.env) (fenv:env clos).
-
-Hypothesis fenv_ok : forall x M,
-  binds x M E' ->
-  exists cl, binds x cl fenv /\
-    has_scheme_vars gc {} empty empty (clos2trm cl) M.
-
-Lemma concat_empty : forall (A:Set) (K:env A), empty & K = K.
-Proof. intros; symmetry; apply (app_nil_end K). Qed.
-
-Lemma has_scheme_from_vars' : forall t M,
-  has_scheme_vars gc {} empty empty t M ->
-  kenv_ok K' -> env_ok E' ->
-  has_scheme gc K' E' t M.
-Proof.
-  clear fenv_ok.
-  intros.
-  apply (@has_scheme_from_vars gc (dom K')).
-  intro; intros.
-  replace K' with (empty & K') by apply concat_empty.
-  apply typing_weaken_kinds.
-    replace E' with (empty & E' & empty) by (simpl; apply concat_empty).
-    apply typing_weaken.
-      simpl.
-      apply* H.
-    simpl. rewrite* concat_empty.
-  assert (fresh {} (sch_arity M) Xs) by auto.
-  puts (H _ H3).
-  rewrite concat_empty.
-  rewrite concat_empty in H4.
-  apply* kenv_ok_concat.
-  rewrite* dom_kinds_open_vars.
-  apply* fresh_disjoint.
-Qed.
 
 Theorem eval_sound : forall h fl xs benv K E t T,
   fresh (dom E) (length benv) xs ->
